Create a generator for next_node behavior given spanning trees

NetworkConfigurations.v
@@ -1,5 +1,9 @@
+Require Import Coq.Lists.List.
+Require Import Coq.Program.Equality.
+
 Section Node.
   Variable Node : Set.
+
   Record flow := {
     Src : Node;
     Dest : Node
@@ -27,63 +31,340 @@ Section Node.
       policy flow = true
         -> exists path, is_next_node_path next path flow.(Src) flow.(Dest);
 
-    no_dead_ends : forall src dest hop_target,
+    no_black_holes : forall src dest hop_target,
       next src dest hop_target
         -> exists path, is_next_node_path next path hop_target dest;
 
     all_paths_acyclic : forall node path,
       is_next_node_path next path node node -> path = nil
   }.
+
+  Fixpoint is_path_in_topology (topology : network_topology) src dest path :=
+    match path with
+    | nil => src = dest
+    | cons hop_target cdr =>
+      topology src hop_target /\
+      is_path_in_topology topology hop_target dest cdr
+    end.
+
+  Record behaved_topology (topology : network_topology) := {
+    connected : forall n1 n2,
+      exists path, is_path_in_topology topology n1 n2 path;
+    undirected : forall n1 n2,
+      topology n1 n2 -> topology n2 n1;
+    no_self_loops : forall n,
+      ~topology n n;
+  }.
+
+  Fixpoint contains_no_duplicates {A} (l : list A) :=
+    match l with
+    | nil => True
+    | cons car cdr => ~In car cdr /\ contains_no_duplicates cdr
+    end.
+
+  Definition next_node_generator := network_topology -> network_policy -> next_node.
+
+  Definition next_node_generator_valid (generator : next_node_generator) (topology_filter : network_topology -> Prop) := forall topology policy,
+    topology_filter topology
+      -> next_node_valid topology policy (generator topology policy).
+
+  Record is_spanning_tree (topology reduced_topology : network_topology) := {
+    is_subgraph : forall n1 n2,
+      reduced_topology n1 n2 -> topology n1 n2;
+    is_tree : forall src dest,
+      exists! path,
+        is_path_in_topology reduced_topology src dest path /\
+        contains_no_duplicates (cons src path)
+  }.
+
+  Definition spanning_tree_next_node_generator' topology (_ : network_policy) src dest target :=
+    exists path,
+      is_path_in_topology topology src dest path /\
+      contains_no_duplicates (src :: path) /\
+      match path with
+      | nil => False
+      | car :: _ => car = target
+      end.
+
+  Lemma spanning_tree_next_node_generator'_valid : forall topology reduced_topology policy,
+    is_spanning_tree topology reduced_topology
+      -> next_node_valid reduced_topology policy (spanning_tree_next_node_generator' reduced_topology policy).
+  Proof.
+    intros.
+    constructor; intros.
+    unfold spanning_tree_next_node_generator' in H0.
+    destruct H0.
+    destruct H0.
+    destruct H1.
+    destruct x.
+    tauto.
+    subst.
+    simpl in H0.
+    destruct H0.
+    assumption.
+    destruct flow0.
+    simpl.
+    apply is_tree with (src := Src0) (dest := Dest0) in H.
+    destruct H.
+    unfold unique in H.
+    apply proj1 in H.
+    destruct H.
+    exists x.
+    clear H0.
+    dependent induction x generalizing Src0.
+    assumption.
+    simpl.
+    constructor.
+    exists (cons a x).
+    tauto.
+    simpl in H, H1.
+    apply IHx; simpl; tauto.
+    apply is_tree with (src := src) (dest := dest) in H.
+    unfold spanning_tree_next_node_generator' in H0.
+    destruct H0.
+    destruct H0.
+    destruct H1.
+    destruct x.
+    tauto.
+    subst.
+    exists x.
+    destruct H.
+    destruct H.
+    destruct H.
+    clear H2.
+    simpl in H0, H1.
+    destruct H0, H1.
+    clear H0.
+    dependent induction x generalizing hop_target.
+    simpl in H2.
+    simpl.
+    assumption.
+    simpl.
+    constructor.
+    exists (cons a x).
+    constructor; try assumption.
+    constructor; try assumption.
+    reflexivity.
+    simpl in H4.
+    destruct H4.
+    destruct H4.
+    simpl in H2.
+    destruct H2.
+    apply IHx; try tauto.
+    unfold not.
+    intros.
+    destruct H7; subst.
+    apply H1.
+    simpl.
+    tauto.
+    apply H1.
+    simpl.
+    tauto.
+    apply is_tree with (src := node) (dest := node) in H.
+    destruct H.
+    assert (x = nil).
+    unfold unique in H.
+    destruct H.
+    apply H1.
+    constructor.
+    constructor.
+    simpl.
+    tauto.
+    subst.
+    simpl in H.
+    destruct path; try reflexivity.
+    exfalso.
+    simpl in H0.
+    destruct H0.
+    destruct H0.
+    destruct H0.
+    destruct H2.
+    unfold unique in H.
+    destruct H.
+    assert (nil = x); subst; try tauto.
+    destruct x; try tauto.
+    subst.
+    simpl in H0.
+    apply H4.
+    constructor; assumption.
+  Qed.
+
+  Lemma next_node_subgraph_weakening : forall (sparse_topology dense_topology : network_topology) policy next,
+    next_node_valid sparse_topology policy next
+      -> (forall n1 n2, sparse_topology n1 n2 -> dense_topology n1 n2)
+      -> next_node_valid dense_topology policy next.
+  Proof.
+    intros.
+    destruct H.
+    constructor; eauto.
+  Qed.
+
+  Variable make_spanning_tree : network_topology -> network_topology.
+
+  Definition spanning_tree_generator_valid topology_filter := forall topology,
+    topology_filter topology -> is_spanning_tree topology (make_spanning_tree topology).
+
+  Definition spanning_tree_next_node_generator topology policy :=
+    spanning_tree_next_node_generator' (make_spanning_tree topology) policy.
+
+  Theorem spanning_tree_next_node_generator_valid (topology_filter : network_topology -> Prop) :
+    spanning_tree_generator_valid topology_filter
+      -> next_node_generator_valid spanning_tree_next_node_generator topology_filter.
+  Proof.
+    unfold next_node_generator_valid, spanning_tree_next_node_generator.
+    intros.
+    assert (H' := H0).
+    apply H in H0.
+    apply next_node_subgraph_weakening with (sparse_topology := make_spanning_tree topology).
+    apply spanning_tree_next_node_generator'_valid with (topology := topology); eauto.
+    apply is_subgraph; assumption.
+  Qed.
 End Node.
 
 Require Import ZArith.
-Section NatNetworkExample.
-  Local Definition nat_topology src dest := src - dest < 10.
-  Local Definition nat_policy (f : flow nat) := Dest nat f <=? Src nat f.
-  Local Inductive nat_next_node : next_node nat :=
-  | MinusOne : forall next_src dest,
-    next_src >= dest -> nat_next_node (S next_src) dest next_src
-  | MinusTwo : forall next_src dest,
-    next_src >= dest -> nat_next_node (S (S next_src)) dest next_src.
+Section NetworkExample.
+  Local Inductive ExampleVertex :=
+  | A
+  | B
+  | C
+  | D
+  .
 
-  Local Lemma reducing_exists : forall src dest,
-    src >= dest
-      -> exists path, is_next_node_path nat nat_next_node path src dest.
+  (*
+    example_topology:
+
+        B
+      / | \
+     A  |  D
+      \ | /
+        C
+  *)
+  Local Definition example_topology n1 n2 :=
+    match (n1, n2) with
+    | (A, B) | (B, A) => True
+    | (A, C) | (C, A) => True
+    | (B, C) | (C, B) => True
+    | (B, D) | (D, B) => True
+    | (C, D) | (D, C) => True
+    | _ => False
+    end.
+
+  (*
+    example_spanning_tree:
+
+        B
+      /   \
+     A     D
+      \
+        C
+  *)
+
+  Local Definition example_spanning_tree n1 n2 :=
+    match (n1, n2) with
+    | (A, B) | (B, A) => True
+    | (A, C) | (C, A) => True
+    | (B, D) | (D, B) => True
+    | _ => False
+    end.
+
+  Local Definition make_example_spanning_tree (_ : network_topology ExampleVertex) := example_spanning_tree.
+
+  Local Definition example_policy (_ : flow ExampleVertex) := true.
+
+  Local Definition next : next_node ExampleVertex :=
+    spanning_tree_next_node_generator ExampleVertex make_example_spanning_tree example_topology example_policy.
+
+  Ltac t := match goal with
+  | [ n : ExampleVertex |- False ] => destruct n
+  | [ Hx : _ -> False |- False ] => apply Hx
+  | [ n : ExampleVertex |- ?n = ?n \/ _ ] => apply or_introl; reflexivity
+  | [ n : ExampleVertex |- _ \/ _ ] => apply or_intror
+  | [ Hx : _ |- In _ _ ] => exfalso
+  end.
+
+  Lemma long_paths_have_duplicates : forall (path : list ExampleVertex),
+    length path < 5 \/ ~contains_no_duplicates path.
   Proof.
     intros.
-    induction src.
-    assert (dest = 0) by omega; subst.
-    exists nil.
-    reflexivity.
-    assert (dest <= src \/ dest = S src) by omega.
-    case H0; intros.
-    assert (H' := H1).
-    apply IHsrc in H1.
-    destruct H1.
-    exists (cons src x).
-    simpl.
-    apply conj; try assumption.
-    constructor.
-    omega.
-    subst.
-    exists nil.
-    reflexivity.
+    destruct path.
+    apply or_introl; simpl; omega.
+    destruct path.
+    apply or_introl; simpl; omega.
+    destruct path.
+    apply or_introl; simpl; omega.
+    destruct path.
+    apply or_introl; simpl; omega.
+    destruct path.
+    apply or_introl; simpl; omega.
+    apply or_intror.
+    unfold contains_no_duplicates.
+    unfold not.
+    intros.
+    simpl in H.
+    destruct e, e0, e1, e2, e3; tauto.
   Qed.
 
-  Local Theorem nat_next_node_valid : next_node_valid nat nat_topology nat_policy nat_next_node.
+  Definition get_example_path n1 n2 :=
+    match (n1, n2) with
+    | (A, A) | (B, B) | (C, C) | (D, D) => nil
+    | (A, B) | (D, B) => cons B nil
+    | (C, B) => cons A (cons B nil)
+    | (B, A) | (C, A) => cons A nil
+    | (D, A) => cons B (cons A nil)
+    | (A, C) => cons C nil
+    | (B, C) => cons A (cons C nil)
+    | (D, C) => cons B (cons A (cons C nil))
+    | (B, D) => cons D nil
+    | (A, D) => cons B (cons D nil)
+    | (C, D) => cons A (cons B (cons D nil))
+    end.
+
+  Lemma negation_distribution : forall (P1 P2 : Prop), ~(P1 \/ P2) -> ~P1 /\ ~P2.
   Proof.
-    constructor; intros.
-    unfold nat_topology.
-    inversion H; omega.
-    unfold nat_policy in H.
-    apply Nat.leb_le in H.
-    apply reducing_exists.
-    omega.
-    inversion H; apply reducing_exists; assumption.
-    destruct path.
-    reflexivity.
-    simpl in H.
-    destruct H.
-    inversion H; omega.
+    tauto.
   Qed.
-End NatNetworkExample.
+
+  Local Theorem validity : next_node_valid ExampleVertex example_topology example_policy next.
+  Proof.
+    assert (next_node_generator_valid ExampleVertex (fun _ _ => next) (fun t => t = example_topology)); try auto.
+    apply spanning_tree_next_node_generator_valid.
+    unfold spanning_tree_generator_valid.
+    intros.
+    unfold make_example_spanning_tree.
+    subst.
+    constructor.
+    intros; destruct n1, n2; try constructor; inversion H.
+    intros.
+    unfold unique.
+    exists (get_example_path src dest).
+    apply conj.
+    apply conj.
+    unfold example_spanning_tree.
+    destruct src, dest; simpl; tauto.
+    destruct src, dest; simpl; repeat match goal with
+    | [ H : _ \/ _ |- _ ] => destruct H
+    | [ |- _ /\ _ ] => constructor
+    | [ |- ~_ ] => unfold not; intros
+    | _ => tauto
+    end; discriminate.
+    intros.
+    destruct H.
+    assert (length x' < 5 \/ ~contains_no_duplicates x') by (apply long_paths_have_duplicates).
+    simpl in H0.
+    destruct H1; try tauto.
+    unfold get_example_path.
+    unfold is_path_in_topology, example_spanning_tree in H.
+    destruct src, dest; repeat match goal with
+    | _ => reflexivity
+    | _ => discriminate
+    | [ H : _ /\ _ |- _ ] => destruct H
+    | [ H : ~(_ \/ _) |- _ ] => apply negation_distribution in H
+    | [ e : ExampleVertex |- _ ] => destruct e; try tauto
+    | [ H : length (_ :: _ :: _ :: _ :: _ :: _) < 5 |- _ ] => simpl in H; omega
+    | [ H : contains_no_duplicates (_ :: _) |- _ ] => simpl in H
+    | [ H : ~In _ (_ :: _) |- _ ] => simpl in H
+    | [ x' : list ExampleVertex |- _ ] => destruct x'
+    | _ => tauto
+    end.
+  Qed.
+End NetworkExample.
